have cut the refinement for update_entries in 4

proof/Refinement.v
@@ -3,10 +3,13 @@ Import ListNotations.
 Require Import Coq.Bool.Bool.
 Require Import Omega.
 Require Import Lia.
+Require Import FunctionalExtensionality.
 From Scheduler.Proof Require Import Lib Assumptions JobsAxioms EdfPolicy FunctionalEdf Hoare EdfPolicy.
 From Scheduler.Model Require Import Monad AbstractTypes AbstractFunctions.
-From Scheduler.SchedulerMockup Require Import Jobs.
-From Scheduler Require Import EDF.
+From Scheduler.SchedulerMockup Require Import Jobs Entry JobSet CNat CBool CRet State.
+From Scheduler.PartitionMockup Require  Import Primitives.
+From Scheduler Require  Import EDF.
+
 
 Module RefinementMod (J :JobsAxiomsMod).
  Import J.
@@ -24,11 +27,199 @@ Definition E :  Env := (fun k =>
                                     (Jobs j).(budget)
                                     (Jobs j).(deadline))          
                                 (jobs_arriving_at k))).
+(* decomposing the update_entry function in 3 smaller units *)
+
+
+Definition read_inputs  :=
+  do new_jobs <- jobs_arriving N ; (* get all jobs arriving at current time, having id < N *)
+  do finished <- job_terminating;  (* does a job finish at current time ? *)
+  do expired <- job_expired;       (* is the job expired ? *)
+  do late <- job_late ;            (* did the job exceed its deadline ?*)
+  ret (new_jobs, finished,expired,late).
+
+Definition update_first_entry (finished expired : CBool) :=
+  do not_expired <- not expired;
+  do finished_and_not_expired <- and finished not_expired ;
+  (if finished_and_not_expired then (* i remove its entry (NB the first one) from active list*)
+    remove_first_active_entry
+  else
+    ret tt).
+
+Definition add_new_entries (new_jobs : JobSet) :=  
+  do new_jobs_length <- get_length new_jobs ;
+  insert_new_entries new_jobs new_jobs_length.
+
+Definition write_output (late : CBool) :=
+  do running_entry_id <- get_running ; (* obtain id of the running job (possibly none) from head of active list*)
+  do no_running_entry <- is_default_nat running_entry_id ;
+  do ret_value <- make_ret_type no_running_entry late running_entry_id ;
+  ret ret_value.
+
+
+Definition decomposed_update_entries :=
+  do tuple <- read_inputs;
+  match tuple with (new_jobs, finished,expired,late) =>
+    update_first_entry finished expired ;;
+    add_new_entries new_jobs ;;
+    write_output late
+  end.
+ 
+
+Lemma decomposition_correct :
+     update_entries = decomposed_update_entries .
+Proof.
+ unfold decomposed_update_entries, update_entries, read_inputs, update_first_entry, add_new_entries, write_output in *.
+ rewrite bind_bind.
+ f_equal.
+ extensionality new_jobs.
+ rewrite bind_bind.
+ f_equal.
+ extensionality finished.
+ rewrite bind_bind.
+ f_equal.
+ extensionality expired.
+  rewrite bind_bind.
+ f_equal.
+Qed.
+
+Definition functional_read_inputs (s : State) :=
+    let  l :=
+     filter (fun j =>  j <? N) (jobs_arriving_at s.(now))  in                                     
+let b := 
+     match hd_error s.(active) with
+     | Some e =>
+         let j := Jobs (id e) in
+         (cnt e <=? budget j - duration j)
+     | None => false
+     end
+in
+let b' :=  match hd_error s.(active) with
+     | Some e =>
+         cnt e =? 0
+     | None => false
+           end
+in
+let b'' :=  match hd_error s.(active) with
+     | Some e =>
+         del e =? 0
+     | None => false
+           end
+in
+( (l,b,b',b''), s).
+
+Definition functional_update_first_entry (s : State) (b b' : bool) :=
+  let active1 := if b && (negb b') then tl s.(active) else s.(active) in
+  (tt,mk_State s.(now) active1).
+
+Definition functional_add_new_entries(s:State) (l : list nat) :=
+ let active2 :=
+       insert_all _
+         (fun e1 e2 : Entry =>
+          deadline (Jobs (id e1)) <=? deadline (Jobs (id e2)))
+         (map
+            (fun j  =>
+             {|
+             id :=  j;
+             cnt := budget (Jobs j);
+             del := S (deadline (Jobs j) - (arrival (Jobs j))) |}) l) s.(active) in
+ (tt,mk_State s.(now) active2).
+
+
+Definition functional_write_output (s : State) (b'' : bool) :=
+   (match s.(active) with
+     | [] => (None,b'')
+     | e :: _ => (Some (id e), b'')
+  end,  mk_State  s.(now) s.(active)).
+
+Definition functional_decomposed_update_entries(s : State) :=
+  let (tuple,s') :=  functional_read_inputs s in
+  match tuple with (l, b,b',b'') =>
+    let (_,s'') := functional_update_first_entry  s' b b' in
+    let (_,s''') := functional_add_new_entries s'' l in
+    functional_write_output s''' b'' 
+  end.
+
+
+Lemma functional_decomposition_correct :
+     functional_update_entries = functional_decomposed_update_entries .
+Proof.
+  auto.
+Qed.
+
+
+
+Lemma functional_read_inputs_refines_monadic :  forall r s0 s,
+   read_inputs E s0 = (r,s) ->  functional_read_inputs s0 = (r,s).
+Admitted.
+
+
+Lemma functional_update_first_entry_refines_monadic :  forall b b' r s0 s,
+    update_first_entry b b' E s0 = (r,s) ->
+    functional_update_first_entry s0 b b'  = (r,s).
+Admitted.
+
+
+Lemma functional_add_new_entries_refines_monadic :  forall l r s0 s,
+    add_new_entries l E s0 = (r,s) ->
+    functional_add_new_entries s0 l  = (r,s).
+Admitted.
+
+
+Lemma functional_write_output_refines_monadic :  forall b'' r s0 s,
+    write_output b'' E s0 = (r,s) ->
+    functional_write_output s0 b''  = (r,s).
+Admitted.
+
 
 Lemma functional_update_entries_refines_monadic :  forall r s0 s,
    update_entries E s0 = (r,s) ->  functional_update_entries s0 = (r,s).
-Admitted.
+Proof.
+  intros r s0 s Hu.
+  
+rewrite decomposition_correct in Hu.
+rewrite functional_decomposition_correct.
+unfold  decomposed_update_entries, bind, ret in Hu.
+unfold functional_decomposed_update_entries.
+rewrite <- Hu.
+clear Hu r s. 
+remember (functional_read_inputs s0) as fri.
+destruct fri as (r,s).
+remember (read_inputs E s0) as ri.
+destruct ri as (r',s').
+symmetry in Heqri.
+generalize Heqri  ; intro Heqri_cp.
+rewrite <- functional_read_inputs_refines_monadic with (s0 := s0) in Heqri ; auto.
+assert (Heq  : (r,s) = (r',s') ) ; [congruence | ].
+injection Heq ; intros ; subst.
+clear s0 Heq Heqri Heqri_cp Heqfri.
+destruct r' as (((l & b) & b') & b'').
+remember (functional_update_first_entry s' b b') as fri.
+destruct fri as (r,s).
+remember (update_first_entry b b' E s') as ri.
+destruct ri as (r'',s'').
+symmetry in Heqri.
+generalize Heqri  ; intro Heqri_cp.
+erewrite <- functional_update_first_entry_refines_monadic with (s0 := s') in Heqri ; eauto.
+assert (Heq  : (r,s) = (r'',s'') ) ; [congruence | ].
+injection Heq ; intros ; subst.
+clear s' Heq Heqri Heqri_cp Heqfri r''.
 
+remember (functional_add_new_entries s'' l) as fri.
+destruct fri as (r,s).
+remember (add_new_entries l E s'') as ri.
+destruct ri as (r',s').
+symmetry in Heqri.
+generalize Heqri  ; intro Heqri_cp.
+erewrite <- functional_add_new_entries_refines_monadic with (s0 := s'') in Heqri ; eauto.
+assert (Heq  : (r,s) = (r',s') ) ; [congruence | ].
+injection Heq ; intros ; subst.
+clear  Heq Heqri Heqri_cp Heqfri r' s'' b b' l.
+
+
+remember (write_output b'' E s') as ri.
+destruct ri as (r'',s'').
+erewrite functional_write_output_refines_monadic; eauto.
+Qed.
 
 
 Lemma functional_update_counters_refines_monadic :  forall r s0 s,
@@ -105,7 +296,6 @@ cbn in *.
    unfold CNat.zero in *.
   case_eq ( Init.Nat.pred (cnt e) =? 0); intro Hcas; rewrite Hcas in *.
   2 :{
-
     injection Heq_s' ; intros; subst.
     auto.
   }
